Add `substFn` helper for `subst₁`; update call sites

Lean4Axiomatic/AbstractAlgebra/Substitutive.lean
@@ -53,6 +53,24 @@ class Substitutive₁
 export Substitutive₁ (subst₁)
 
 /--
+Convenience function for the unary generalized substitution property, for a
+predicate `f`.
+
+Type inference for `subst₁` gets stuck when the output relation is `(· → ·)`;
+this helper works around that issue by hardcoding the argument.
+
+See `subst₁` for further documentation.
+
+**Named parameters**
+- `α`: The `Sort` of `f`'s input parameter.
+- `f`: The unary predicate that obeys the generalized substitution property.
+- `rα`: A binary relation on `f`'s input values.
+- See `subst₁` for documentation on the remaining parameters.
+-/
+abbrev substFn {α : Sort u} {f : α → Prop} {rα : α → α → Prop} :=
+  @subst₁ α (β := Prop) f rα (rβ := (· → ·))
+
+/--
 Class for types and operations that satisfy the unary generalized injective
 property.
 
